cilc2

coq/cilc2/clc_soundness.v
@@ -1,17 +1,424 @@
 From mathcomp Require Import ssreflect ssrbool eqtype ssrnat seq.
 From Coq Require Import ssrfun Utf8 Classical.
-Require Import AutosubstSsr ARS 
+Require Import AutosubstSsr ARS
   clc_context clc_ast clc_confluence clc_subtype clc_typing
-  clc_weakening clc_substitution clc_inversion clc_validity.
+  clc_weakening clc_substitution clc_inversion clc_arity_spine
+  clc_validity clc_typing_spine clc_respine clc_iota_lemma.
 
 Set Implicit Arguments.
 Unset Strict Implicit.
 Unset Printing Implicit Defensive.
 
+Lemma arity_step s A A' : arity s A -> A ~> A' -> arity s A'.
+Proof.
+  move=>ar. elim: ar A'=>{A}.
+  move=> l A' st. inv st.
+  move=> A0 B a ih A' st. inv st.
+  constructor; eauto.
+  constructor; eauto.
+Qed.
+
+Inductive n_beta k (σ : var -> term) x :=
+| N_beta :
+  k < x.+1 ->
+  (forall i, i < k -> σ i = (Var i)) ->
+  noccurs x (σ k) ->
+  (forall i, k < i -> (σ i).[ren (+1)] = Var i) ->
+  n_beta k σ x.
+
+Lemma noccurs_n_beta x m : noccurs x m -> n_beta 0 (m .: ids) x.
+Proof.
+  move=>no. constructor; eauto.
+  move=>[|i] h; inv h.
+  move=>[|i] h; inv h.
+  asimpl; eauto.
+Qed.
+
+Lemma n_beta_up k x σ : n_beta k σ x -> n_beta k.+1 (up σ) x.+1.
+Proof.
+  move=>[lt h1 h2 h3].
+  constructor; eauto.
+  move=>[|i h]; eauto; asimpl.
+  have/h1->//: i < k by eauto.
+  asimpl. apply: noccurs_up; eauto.
+  move=>[|i] h; asimpl. inv h.
+  replace (σ i).[ren (+2)] with (σ i).[ren (+1)].[ren (+1)] by autosubst.
+  have/h3->//: k < i by eauto.
+Qed.
+
+Lemma lt_false x y : x < y -> y < x.+1 -> False.
+Proof.
+  elim: x y.
+  move=>[|y] h1 h2; inv h1. inv h2.
+  move=>n ih [|y] h1 h2. inv h1.
+  apply: ih; eauto.
+Qed.
+
+Lemma noccurs_beta k x m σ : noccurs x.+1 m -> n_beta k σ x -> noccurs x m.[σ].
+Proof with eauto using n_beta, n_beta_up.
+  move e:(x.+1)=>i no. move: i m no σ k x e.
+  apply: noccurs_ind_nested=>//=.
+  all: try solve[intros; subst; eauto using noccurs, n_beta, n_beta_up ].
+  move=>x y neq σ k x0 e [leq h1 no h3]; subst.
+  { have[h|h|h]:=ltngtP k y.
+    have{}h:=h3 _ h.
+    destruct (σ y)=>//. inv h.
+    constructor...
+    rewrite h1...
+    constructor.
+    move=>e; subst.
+    apply: lt_false...
+    subst... }
+  move=>x A Cs s nA ih nCs ihCs σ k x0 e nb; subst.
+  { constructor...
+    elim: ihCs. constructor.
+    move=>C Cs' hd tl ihc.
+    constructor... }
+  move=>x m Q Fs nm ihm nQ ihQ nFs ihFs σ k x0 e nb; subst.
+  { constructor...
+    elim: ihFs. constructor.
+    move=>C Cs' hd tl ihc.
+    constructor... }
+Qed.
+
+Lemma noccurs_spine' x h1 h2 ms :
+  noccurs x (spine' h1 ms) -> noccurs x h2 -> noccurs x (spine' h2 ms).
+Proof.
+  move e:(spine' h1 ms)=> n no. move: x n no h1 h2 ms e.
+  apply: noccurs_ind_nested; move=>*;
+  match goal with
+  | [ H : spine' _ ?ms = _ |- _ ] =>
+    destruct ms; simpl; simpl in H; inv H; eauto
+  end.
+  constructor; eauto.
+Qed.
+
+Lemma noccurs_spine x h1 h2 ms :
+  noccurs x (spine h1 ms) -> noccurs x h2 -> noccurs x (spine h2 ms).
+Proof.
+  rewrite! spine_spine'_rev=> noSp no.
+  apply: noccurs_spine'; eauto.
+Qed.
+
+Lemma noccurs_step x m n : noccurs x m -> m ~> n -> noccurs x n.
+Proof with eauto using noccurs, noccurs_beta, noccurs_n_beta.
+  move=> no. move: x m no n.
+  apply: noccurs_ind_nested;
+  try solve [intros;
+             match goal with
+             | [ H : step _ _ |- _ ] =>
+                 inv H; eauto using noccurs
+             end].
+  move=>x m n nm ihm nn ihn n0 st. inv st... inv nm...
+  move=>x A Cs s nA ihA nCs ihCs n st.
+  { inv st...
+    constructor...
+    elim: H3 ihCs nCs.
+    move=>m m' ls st h1 h2. inv h1. inv h2. constructor...
+    move=>m ls ls' h1 h2 h3 h4. inv h3. inv h4. constructor... }
+  move=>x m Q Fs nm ihm nQ ihQ nFs ihFs n st.
+  { inv st...
+    constructor...
+    elim: H3 ihFs nFs.
+    move=>m0 m' ls st h1 h2. inv h1. inv h2. constructor...
+    move=>m0 ls ls' h1 h2 h3 h4. inv h3. inv h4. constructor...
+    apply: noccurs_spine...
+    elim: H3 nFs.
+    move=>m ls nFs. inv nFs...
+    move=>n m m' ls ig ih nFs. inv nFs... }
+  move=>x A m nA ihA nm ihm n st. inv st...
+Qed.
+
+Lemma head_spine'_step h h' ms : h ~> h' -> spine' h ms ~> spine' h' ms.
+Proof.
+  elim: ms h h'; eauto.
+  move=> h ms ih h1 h2 st; simpl.
+  constructor; eauto.
+Qed.
+
+Lemma head_spine'_conv h h' ms : h === h' -> spine' h ms === spine' h' ms.
+Proof.
+  elim: ms h h'; eauto.
+  move=> h ms ih h1 h2 e; simpl.
+  apply: conv_app; eauto.
+Qed.
+
+Lemma head_spine_step h h' ms : h ~> h' -> spine h ms ~> spine h' ms.
+Proof.
+  rewrite! spine_spine'_rev=>st.
+  apply: head_spine'_step; eauto.
+Qed.
+
+Lemma head_spine_conv h h' ms : h === h' -> spine h ms === spine h' ms.
+Proof.
+  rewrite! spine_spine'_rev=>st.
+  apply: head_spine'_conv; eauto.
+Qed.
+
+Lemma var_spine'_step x ms C :
+  spine' (Var x) ms ~> C -> All1 (noccurs x) ms ->
+  exists ms', C = spine' (Var x) ms' /\ All1 (noccurs x) ms'.
+Proof.
+  elim: ms x C=>//=.
+  move=> x C st. inv st.
+  move=> a l ih x C st no.
+  inv no. inv st.
+  destruct l; inv H0.
+  have[ms'[e no]]:=ih x m' H4 H2; subst.
+  exists (a :: ms')=>//=. repeat constructor; eauto.
+  exists (n' :: l)=>//=. repeat constructor; eauto.
+  apply: noccurs_step; eauto.
+Qed.
+
+Lemma noccurs_All1_cat x ms ns :
+  All1 (noccurs x) ms -> All1 (noccurs x) ns -> All1 (noccurs x) (ms ++ ns).
+Proof with eauto using All1. move=>no. elim: no ns... Qed.
+
+Lemma noccurs_All1_rev x ms : All1 (noccurs x) ms -> All1 (noccurs x) (rev ms).
+Proof with eauto using All1.
+  elim: ms=>//=.
+  move=>m ms ih nms. inv nms.
+  have{H2}ih:=ih H2.
+  replace (m :: ms) with ([:: m] ++ ms) by eauto.
+  rewrite rev_cat.
+  apply: noccurs_All1_cat...
+Qed.
+
+Lemma var_spine_step x ms C :
+  spine (Var x) ms ~> C -> All1 (noccurs x) ms ->
+  exists2 ms', C = spine (Var x) ms' & All1 (noccurs x) ms'.
+Proof.
+  rewrite! spine_spine'_rev.
+  move=>st/noccurs_All1_rev no.
+  have[ms' [h1 h2]]:=var_spine'_step st no.
+  exists (rev ms').
+  rewrite spine_spine'_rev. rewrite revK; eauto.
+  apply: noccurs_All1_rev; eauto.
+Qed.
+
+Lemma pos_step x A B : pos x A -> A ~> B -> pos x B.
+Proof.
+  move=> p. elim: p B=>{A x}.
+  move=> x ms no B st.
+  have[ms'[e no']]:=var_spine_step st no; subst.
+  constructor; eauto.
+  move=>x A B s r t n p ih B' st. inv st.
+  constructor; eauto.
+  apply: noccurs_step; eauto.
+  constructor; eauto.
+Qed.
+
+Lemma constr_step x s C C' : constr x s C -> C ~> C' -> constr x s C'.
+Proof.
+  move=>c. elim: c C'=>{C x s}.
+  move=>x s ms nms C' st.
+  { have[ms' e nms']:=var_spine_step st nms; subst.
+    constructor; eauto. }
+  move=>s t x A B leq pA nB cB ih C' st. inv st.
+  { apply: constr_pos; eauto.
+    apply: pos_step; eauto. }
+  { apply: constr_pos; eauto.
+    apply: noccurs_step; eauto. }
+  move=>s t x A B leq nB cB ih C' st. inv st.
+  { apply: constr_pi; eauto.
+    apply: noccurs_step; eauto. }
+  { apply: constr_pi; eauto. }
+Qed.
+
+Lemma iget_step i Cs Cs' C :
+  iget i Cs C -> One2 step Cs Cs' ->
+  exists2 C', C === C' & iget i Cs' C'.
+Proof.
+  move=>ig h. elim: h i ig=>{Cs Cs'}.
+  move=>m m' ls st i ig. inv ig.
+  { exists m'; repeat constructor; eauto. apply: conv1; eauto. }
+  { exists C; repeat constructor; eauto. }
+  move=>m ls ls' st ih i ig. inv ig.
+  { exists C; repeat constructor; eauto. }
+  { have[C' cC ig]:=ih _ H3.
+    exists C'; repeat constructor; eauto. }
+Qed.
+
+Lemma respine0_step Q Q' C : Q ~> Q' -> respine0 Q C ~> respine0 Q' C.
+Proof with eauto using step. elim: C Q Q'... Qed.
+
+Lemma respine_step k s Q Q' c C :
+  Q ~> Q' ->
+  (respine k s Q c C).1 = (respine k s Q' c C).1 /\
+  (respine k s Q c C).2 ~> (respine k s Q' c C).2.
+Proof with eauto using step, respine0_step.
+  elim: C k s Q Q' c.
+  move=>x [|] s Q Q' c st//=...
+  move=>s l [|] s0 Q Q' c st//=...
+  move=>A ihA B ihB s r t [|] s0 Q Q' c st//=.
+  { pose proof (step_subst (ren (+1)) st) as st'.
+    pose proof (ihB U s0 _ _ (App c.[ren (+1)] (Var 0)) st') as [h1 h2].
+    remember (respine U s0 Q.[ren (+1)] (App c.[ren (+1)] (Var 0)) B) as p1.
+    remember (respine U s0 Q'.[ren (+1)] (App c.[ren (+1)] (Var 0)) B) as p2.
+    destruct p1.
+    destruct p2.
+    simpl.
+    split; eauto.
+    simpl in h1; subst.
+    simpl in h2.
+    constructor; eauto. }
+  { pose proof (step_subst (ren (+1)) st) as st'.
+    pose proof (ihB L s0 _ _ (App c.[ren (+1)] (Var 0)) st') as [h1 h2].
+    remember (respine L s0 Q.[ren (+1)] (App c.[ren (+1)] (Var 0)) B) as p1.
+    remember (respine L s0 Q'.[ren (+1)] (App c.[ren (+1)] (Var 0)) B) as p2.
+    destruct p1.
+    destruct p2.
+    simpl.
+    split; eauto.
+    simpl in h1; subst.
+    simpl in h2.
+    constructor; eauto. }
+  move=>A ihA m ihm s t [|] s0 Q Q' c st//=...
+  move=>m ihm n ihn [|] s Q Q' c st//=...
+  move=>A ihA Cs s [|] s0 Q Q' c st//=...
+  move=>i m ihm [|] s Q Q' c st//=...
+  move=>m ihm Q ihQ Fs [|] s Q0 Q' c st//=...
+  move=>A ihA m ihm [|] s Q Q' c st//=...
+Qed.
+
+Lemma mkcase_step k s I Q Q' c C :
+  Q ~> Q' ->
+  (mkcase k s I Q c C).1 = (mkcase k s I Q' c C).1 /\
+  (mkcase k s I Q c C).2 ~> (mkcase k s I Q' c C).2.
+Proof.
+  move=>st. unfold mkcase.
+  apply: respine_step; eauto.
+Qed.
+
+Inductive sub_list : nat -> list term -> list term -> Prop :=
+| sub_list_O xs : sub_list 0 xs xs
+| sub_list_S x xs ys n :
+  sub_list n xs ys -> sub_list n.+1 (x :: xs) ys.
+
+Lemma sub_list_iget i XS x xs :
+  sub_list i XS (x :: xs) -> iget i XS x.
+Proof.
+  move e:(x :: xs)=> ys sb.
+  elim: sb x xs e=>{i XS ys}.
+  move=>xs x xs0 e; subst. constructor.
+  move=>x xs ys n sbl ih x0 xs0 e; subst.
+  constructor; eauto.
+Qed.
+
+Lemma sub_list_ok i XS x xs :
+  sub_list i XS (x :: xs) -> sub_list i.+1 XS xs.
+Proof.
+  move e:(x :: xs)=> ys sb.
+  elim: sb x xs e=>{i XS ys}.
+  move=>xs s xs0 e; subst. repeat constructor.
+  move=>x xs ys n sbl ih x0 xs0 e; subst.
+  constructor; eauto.
+Qed.
+
+Lemma All2i_strengthen (P : nat -> term -> term -> Prop) Cs Fs Xs n :
+  All2i (fun i F C => P i F C) n Fs Xs ->
+  sub_list n Cs Xs ->
+  All2i (fun i F C => iget i Cs C /\ P i F C) n Fs Xs.
+Proof.
+  move=> a2i. elim: a2i Cs=>{Fs Xs n}.
+  move=>i Cs sbl. constructor.
+  move=>i m m' ls ls' pm hd ih Cs sbl.
+  constructor.
+  move/sub_list_iget in sbl=>//.
+  apply: ih. apply: sub_list_ok; eauto.
+Qed.
+
+Lemma All2i_mkcase_stepQ Γ A Q Q' Fs Cs Xs n k s s' l :
+  let I := Ind A Cs s in
+  s ≤ k ->
+  Q ~> Q' ->
+  arity s A ->
+  [Γ] ⊢ I : A : U ->
+  [Γ] ⊢ Q' : rearity k s' I A : U ->
+  sub_list n Cs Xs ->
+  All2i (fun i F C =>
+    constr 0 s C /\
+    let T := mkcase k s' I Q (Constr i I) C in
+    Γ ⊢ F : T.2 : T.1) n Fs Xs ->
+  All1 (fun C => A :U [Γ] ⊢ C : s @ l : U) Xs ->
+  All2i (fun i F C =>
+    constr 0 s C /\
+    let T := mkcase k s' I Q' (Constr i I) C in
+    Γ ⊢ F : T.2 : T.1) n Fs Xs.
+Proof.
+  move=>I leq st ar tyI tyQ sbl a2i.
+  have{sbl}a2i:=All2i_strengthen a2i sbl. elim: a2i=>{Fs Xs}.
+  constructor.
+  move=>i F C Fs Cs'[ig[cm tym]] hd ih tl. inv tl.
+  constructor; eauto.
+  split; eauto.
+  have h1 : (I .: ids) 0 = Ind A Cs s by eauto.
+  have h2 : [Γ] ⊢ C.[I/] : (s @ l).[I/] : U.
+  { apply: substitution.
+    apply: H1.
+    apply: (re_pure Γ).
+    apply: merge_re_id.
+    eauto. }
+  pose proof (respine_step k s' (Constr i I) C.[I/] st) as [h3 h4].
+  have{}h4 :
+    (respine k s' Q (Constr i I) C.[I/]).2 <:
+    (respine k s' Q' (Constr i I) C.[I/]).2.
+  { apply: conv_sub.
+    apply: conv1; eauto. }
+  have h5 : [Γ] ⊢ Constr i I : C.[I/] : s.
+  { apply: clc_constr; eauto.
+    apply: re_pure. }
+  destruct k.
+  { inv leq.
+    have//=[l0 ty]:=constr_respineU cm ar h1 tyI tyQ h2 h5.
+    unfold mkcase.
+    unfold mkcase in tym.
+    apply: clc_conv.
+    apply: h4.
+    rewrite<-h3.
+    apply: tym.
+    eauto. }
+  { have//=[l0 ty]:=constr_respineL (Constr i I) cm ar h1 tyI tyQ h2.
+    unfold mkcase.
+    unfold mkcase in tym.
+    apply: clc_conv.
+    apply: h4.
+    rewrite<-h3.
+    apply: tym.
+    eauto. }
+Qed.
+
+Lemma All2i_One2_stepF Γ A Q Fs Fs' Cs Cs' n k s s' :
+  let I := Ind A Cs' s in
+  ok Γ ->
+  One2 step Fs Fs' ->
+  All2i (fun i F C =>
+    constr 0 s C /\
+    let T := mkcase k s' I Q (Constr i I) C in
+    Γ ⊢ F : T.2 : T.1) n Fs Cs ->
+  All2i (fun i F C =>
+    constr 0 s C /\ (ok Γ -> forall F',
+    F ~> F' ->
+    let T := mkcase k s' I Q (Constr i I) C in
+    Γ ⊢ F' : T.2 : T.1)) n Fs Cs ->
+  All2i (fun i F C =>
+    constr 0 s C /\
+    let T := mkcase k s' I Q (Constr i I) C in
+    Γ ⊢ F : T.2 : T.1) n Fs' Cs.
+Proof.
+  move=>I wf oFs. elim: oFs Cs n=>{Fs Fs'}.
+  move=>F F' Fs' st Cs n hd tl. inv hd. inv tl.
+  { constructor; eauto.
+    inv H5. split; eauto. }
+  move=>F Fs Fs' oFs ih Cs n hd tl. inv hd. inv tl.
+  { constructor; eauto. }
+Qed.
+
 Theorem subject_step Γ m n A s :
   ok Γ -> Γ ⊢ m : A : s -> m ~> n -> Γ ⊢ n : A : s.
 Proof with eauto using clc_type, step, ok, merge_re_id.
-  move=>wf tp. elim: tp n wf=>{Γ m A s}.
+  move=>wf tp.
+  move: Γ m A s tp n wf. apply: clc_type_ind_nested.
   move=>Γ s l k n o st. inv st.
   move=>Γ A B s r t i k tyA ihA tyB ihB n o st. inv st.
   { move:(ihA _ o H5)=>tyA'.
@@ -63,7 +470,7 @@ Proof with eauto using clc_type, step, ok, merge_re_id.
   { move:(ihm _ H2)=>{}ihm.
     apply: clc_app... }
   { move:(ihn _ H2)=>{}ihn.
-    move:(pi_inv tyP)=>[l[tyA[_ tyB]]].
+    move:(pi_inv tyP)=>[l[tyA[_[_ tyB]]]].
     move:(merge_re_re mrg)=>[e1[e2 e3]].
     destruct s.
     { have mrg' : [Γ1] ∘ Γ2 => [Γ].
@@ -85,146 +492,78 @@ Proof with eauto using clc_type, step, ok, merge_re_id.
       apply: clc_app...
       rewrite<-e2.
       exact: tyB. } }
-  move=>Γ k n o st. inv st.
-  move=>Γ k n o st. inv st.
-  move=>Γ k n o st. inv st.
-  move=>Γ k n o st. inv st.
-  move=>Γ k n o st. inv st.
-  move=>Γ A B s r t i mrg k tyA ihA tyB ihB n o st. inv st.
-  { move:(ihA _ o H5)=>{ihA}tyA'.
-    apply: clc_sigma...
-    destruct s; simpl.
+  move=>Γ A Cs s l k ar cCs tyA ihA tyCs ihCs n wf st. inv st.
+  { apply: clc_conv.
+    apply: conv_sub.
+    apply: conv1i...
+    apply: clc_indd...
+    apply: arity_step...
+    elim: tyCs. constructor.
+    move=>C Cs' tyC hd tl.
+    constructor...
     apply: context_conv.
     apply: conv1i...
-    rewrite<-re_invo.
     rewrite<-pure_re...
-    exact: tyB.
-    exact: tyB. }
-  { destruct s; simpl in tyB.
-    have okA:ok (A :U [Γ]).
-    apply: ty_ok...
-    rewrite<-pure_re...
-    rewrite<-re_invo.
-    rewrite<-pure_re...
-    move:(ihB _ okA H5)=>//=tyB'.
-    apply: clc_sigma...
-    move:(ihB _ (n_ok (re_ok o)) H5)=>//=tyB'.
-    apply: clc_sigma... }
-  move=>Γ1 Γ2 Γ A B m n s r t i k1 k2 mrg
-    tyS ihS tym ihm tyn ihn n0 o st. 
-  move:(merge_context_ok_inv mrg o)=>[o1 o2]. 
-  move:(merge_re_re mrg)=>[e[e1 e2]].
-  move:(sigma_inv tyS)=>[G1[G2[i0[_[mrg0[tyA tyB]]]]]].
-  move:(merge_re_re mrg0)=>[e3[e4 e5]]. inv st.
-  { move:(ihm _ o1 H3)=>{ihm ihS ihn}tym'.
-    rewrite<-re_invo in e4.
-    rewrite<-re_invo in e5.
-    apply:clc_pair...
-    apply:clc_conv.
-    apply:conv_sub.
-    apply:conv_beta.
-    apply:conv1...
-    exact:tyn.
-    destruct s; simpl in tyB.
-    have mrg1:[G2] ∘ Γ1 => [Γ2].
-    rewrite e5 e2 (pure_re k1) e1.
-    apply:merge_re_id.
-    have:=substitution tyB k1 mrg1 tym'. asimpl...
-    have:=substitutionN tyB tym'. 
-    rewrite e5. rewrite<-e2... }
-  { move:(ihn _ o2 H3)=>{ihm ihS ihn}tyn'.
-    apply:clc_pair... }
-  move=>Γ1 Γ2 Γ m n1 n2 A s t i k mrg
-    tym ihm tyA ihA tyn1 ihn1 tyn2 ihn2 n wf st.
-  have[wf1 wf2]:=merge_context_ok_inv mrg wf.
-  have{}ihm:=ihm _ wf1.
-  have{}ihn1:=ihn1 _ wf2.
-  have{}ihn2:=ihn2 _ wf2.
-  have/ihA{}ihA:ok [Either :{s} Γ2].
-  { destruct s; simpl.
-    econstructor.
-    apply: re_ok...
-    apply: clc_either.
-    apply: re_pure.
-    constructor.
-    apply: re_ok... }
-  have[_[e1 e2]]:=merge_re_re mrg.
-  inv st.
-  { have{}ihm:=ihm _ H3.
-    destruct s; simpl in tyA.
-    have mrg':[Γ2] ∘ Γ1 => [Γ].
-    { replace Γ1 with [Γ1].
-      apply: merge_re3. apply: merge_sym...
+    eauto.
+    rewrite<-pure_re... }
+  { apply: clc_indd...
+    elim: H3 cCs=>{Cs Cs' tyCs ihCs}.
+    { move=>C C' Cs' st h. inv h.
+      constructor...
+      apply: constr_step... }
+    { move=>C Cs Cs' oCs ih h. inv h.
+      constructor... }
+    elim: H3 tyCs ihCs=>{Cs Cs' cCs}.
+    { move=>C C' Cs' st h1 h2. inv h1. inv h2.
+      constructor...
+      apply: H3...
+      apply: ty_ok...
       rewrite<-pure_re... }
-    have tymA:=substitution tyA k mrg' tym.
+    { move=>C C' Cs' st ih h1 h2. inv h1. inv h2.
+      constructor... } }
+  move=>Γ A s i C Cs I k ig tyI ih n wf st. inv st. inv H2.
+  { have st : Ind A Cs s ~> Ind A' Cs s.
+    { constructor; eauto. }
+    have{}ih:=ih _ wf st.
+    have[l[_[_[ar[cCs[tyA tyCs]]]]]]:=ind_inv tyI.
+    have[l'[_[_[_[_[tyA' _]]]]]]:=ind_inv ih.
+    have tyC:=iget_All1 ig tyCs.
+    have//=tyCI:=substitution tyC k (merge_pure k) tyI.
     apply: clc_conv.
     apply: conv_sub.
     apply: conv_beta.
     apply: conv1i...
-    apply: clc_case...
-    apply: tymA.
-    have tymA:=substitutionN tyA tym.
+    apply: clc_constr...
     apply: clc_conv.
     apply: conv_sub.
-    apply: conv_beta.
-    apply: conv1i...
-    apply: clc_case...
-    rewrite<-e2... }
-  { have{}ihn1:=ihn1 _ H3.
-    apply: clc_case... }
-  { have{}ihn2:=ihn2 _ H3.
-    apply: clc_case... }
-  { have k1:=left_inv tym.
-    have->//:=merge_pureL mrg k1. }
-  { have k1:=right_inv tym.
-    have->//:=merge_pureL mrg k1. }
-  move=>Γ1 Γ2 Γ m n A s mrg tym ihm tyn ihn n0 o st.
-  move:(merge_context_ok_inv mrg o)=>[o1 o2]. inv st.
-  { move:(ihm _ o1 H2)=>tym'.
-    apply: clc_letin1... }
-  { move:(ihn _ o2 H2)=>tyn'.
-    apply: clc_letin1... }
-  { move:(it_inv tym)=>k.
-    by rewrite (merge_pureL mrg k). }
-  move=>Γ1 Γ2 Γ A B C m n s r t k x i leq key mrg 
-    tym ihm tyC ihC tyn ihn n0 o st.
-  move:(merge_context_ok_inv mrg o)=>[o1 o2]. 
-  move:(validity o1 tym)=>[l tyS].
-  move:(sigma_inv tyS)=>[G1[G2[i0[_[mrg0[tyA tyB]]]]]].
-  move:(merge_re_re mrg)=>[e0[e1 e2]].
-  move:(merge_re_re mrg0)=>[e3[e4 e5]].
-  inv st.
-  { move:(ihm _ o1 H2)=>tym'.
+    apply: conv1...
+    eauto.
+    rewrite<-pure_re...
+    rewrite<-pure_re... }
+  { have st : Ind A Cs s ~> Ind A Cs' s.
+    { constructor... }
+    have{}ih:=ih _ wf st.
+    have[l[_[_[ar[cCs[tyA tyCs]]]]]]:=ind_inv tyI.
+    have[l'[_[_[_[cCs'[tyA' tyCs']]]]]]:=ind_inv ih.
+    have[C' e' ig']:=iget_step ig H4.
+    have tyC:=iget_All1 ig tyCs.
+    have tyC':=iget_All1 ig' tyCs'.
+    have//=tyCI:=substitution tyC k (merge_pure k) tyI.
+    have//=tyCI':=substitution tyC' k (merge_pure k) ih.
+    have h: C.[I/] === C'.[Ind A Cs' s/].
+    { apply: (conv_trans C.[Ind A Cs' s/]).
+      apply: conv_beta. apply: conv1...
+      apply: conv_subst... }
     apply: clc_conv.
     apply: conv_sub.
-    apply: conv_beta.
-    apply: conv1i...
-    apply: clc_letin2...
-    destruct k; simpl in tyC.
-    have mrg1:[Γ2] ∘ Γ1 => [Γ].
-    rewrite e2 (pure_re key) e1.
-    apply:merge_re_id. inv leq.
-    have:=substitution tyC key mrg1 tym.
-    asimpl...
-    have:=substitutionN tyC tym.
-    asimpl. by rewrite e2. }
-  { rewrite<-re_invo in e4.
-    rewrite<-re_invo in e5.
-    have[k1 k2]:=merge_pure_inv mrg0 (re_pure _).
-    have oAB :ok (B :{r} A :{s} Γ2).
-    econstructor.
-    econstructor...
-    rewrite<-e0. rewrite<-e4. rewrite<-pure_re...
-    move:tyB; destruct s=>//=; rewrite e5 e0...
-    move:(ihn _ oAB H2)=>tyn'.
-    apply: clc_letin2... }
-  { rewrite<-re_invo in e4.
-    rewrite<-re_invo in e5.
-    move:(pair_inv tym tyS)=>
-      [G3[G4[->[et[k1[k2[mrg1[tym1 tym2]]]]]]]]; subst.
-    have[G[/merge_sym mrg2 /merge_sym mrg3]]:=merge_splitL mrg mrg1.
-    have:=substitution2 tyn k1 k2 mrg2 mrg3 tym1 tym2.
-    by asimpl. }
+    apply: conv_sym...
+    apply: clc_constr...
+    rewrite<-pure_re... }
+  move=>Γ1 Γ2 Γ A Q s s' k Fs Cs m ms I leq ar key mrg
+    tym ihm tyQ ihQ tyFs ihFs n wf st. inv st.
+  {
+
+  }
   move=>Γ A B m s i sb tym ihm tyB ihB n o st.
   { apply: clc_conv... }
 Qed.
